Split Terms File; Improve (use of) GroundTerm

ExistentialRules/Terms/Basic.lean
@@ -18,486 +18,256 @@ structure SkolemFS (sig : Signature) [DecidableEq sig.V] where
 
 abbrev PreGroundTerm (sig : Signature) [DecidableEq sig.C] [DecidableEq sig.V] := FiniteTree (SkolemFS sig) sig.C
 
-mutual
-
-  def PreGroundTerm.arity_ok {sig : Signature} [DecidableEq sig.C] [DecidableEq sig.V] : FiniteTree (SkolemFS sig) sig.C -> Bool
-  | .leaf _ => true
-  | .inner func ts =>
-    ts.toList.length == func.arity && arity_ok_list ts
-
-  def PreGroundTerm.arity_ok_list {sig : Signature} [DecidableEq sig.C] [DecidableEq sig.V] : FiniteTreeList (SkolemFS sig) sig.C -> Bool
-  | .nil => true
-  | .cons hd tl => arity_ok hd && arity_ok_list tl
-
-end
-
-theorem PreGroundTerm.arity_ok_list_iff_arity_ok_each_mem {sig : Signature} [DecidableEq sig.C] [DecidableEq sig.V] (ts : FiniteTreeList (SkolemFS sig) sig.C) : (∀ t, t ∈ ts.toList -> PreGroundTerm.arity_ok t) ↔ PreGroundTerm.arity_ok_list ts := by
-  cases ts with
-  | nil => simp [arity_ok_list, FiniteTreeList.toList]
-  | cons hd tl =>
-    unfold arity_ok_list
-    simp [FiniteTreeList.toList]
-    intro _
-    apply arity_ok_list_iff_arity_ok_each_mem
-
-section FunctionPathsAndCyclicity
-
-  variable {sig : Signature} [DecidableEq sig.V]
+namespace PreGroundTerm
 
   mutual
 
-    def PreGroundTerm.function_paths : FiniteTree (SkolemFS sig) sig.C -> List (List (SkolemFS sig))
-    | .leaf _ => [[]]
-    | .inner f ts =>
-      match ts with
-      | .nil => [[f]]
-      | _ => (function_paths_list ts).map (fun path => f :: path)
+    def arity_ok {sig : Signature} [DecidableEq sig.C] [DecidableEq sig.V] : FiniteTree (SkolemFS sig) sig.C -> Bool
+    | .leaf _ => true
+    | .inner func ts =>
+      ts.toList.length == func.arity && arity_ok_list ts
 
-    def PreGroundTerm.function_paths_list : FiniteTreeList (SkolemFS sig) sig.C -> List (List (SkolemFS sig))
-    | .nil => []
-    | .cons hd tl => (function_paths hd) ++ (function_paths_list tl)
+    def arity_ok_list {sig : Signature} [DecidableEq sig.C] [DecidableEq sig.V] : FiniteTreeList (SkolemFS sig) sig.C -> Bool
+    | .nil => true
+    | .cons hd tl => arity_ok hd && arity_ok_list tl
 
   end
 
-  mutual
+  theorem arity_ok_list_iff_arity_ok_each_mem {sig : Signature} [DecidableEq sig.C] [DecidableEq sig.V] (ts : FiniteTreeList (SkolemFS sig) sig.C) : (∀ t, t ∈ ts.toList -> PreGroundTerm.arity_ok t) ↔ PreGroundTerm.arity_ok_list ts := by
+    cases ts with
+    | nil => simp [arity_ok_list, FiniteTreeList.toList]
+    | cons hd tl =>
+      unfold arity_ok_list
+      simp [FiniteTreeList.toList]
+      intro _
+      apply arity_ok_list_iff_arity_ok_each_mem
 
-    theorem PreGroundTerm.function_path_elements_are_inner_labels (t : FiniteTree (SkolemFS sig) sig.C) : ∀ (path : List (SkolemFS sig)), path ∈ PreGroundTerm.function_paths t -> ∀f, f ∈ path -> f ∈ t.innerLabels := by
-      intro path path_mem f f_mem
-      cases t with
-      | leaf c =>
-        simp only [function_paths, List.mem_singleton] at path_mem
-        rw [path_mem] at f_mem
-        simp at f_mem
-      | inner func ts =>
-        unfold function_paths at path_mem
-        cases ts with
-        | nil =>
-          rw [List.mem_singleton] at path_mem
-          rw [path_mem] at f_mem
-          rw [List.mem_singleton] at f_mem
-          unfold FiniteTree.innerLabels
-          rw [List.mem_cons]
-          apply Or.inl
-          exact f_mem
-        | cons hd tl =>
-          rw [List.mem_map] at path_mem
-          rcases path_mem with ⟨path', mem, eq⟩
-          rw [← eq] at f_mem
-          rw [List.mem_cons] at f_mem
-          unfold FiniteTree.innerLabels
-          rw [List.mem_cons]
-          cases f_mem with
-          | inl f_mem => apply Or.inl; exact f_mem
-          | inr f_mem =>
-            apply Or.inr
-            exact function_path_elements_are_inner_labels_list (FiniteTreeList.cons hd tl) path' mem f f_mem
-
-    theorem PreGroundTerm.function_path_elements_are_inner_labels_list (ts : FiniteTreeList (SkolemFS sig) sig.C) : ∀ (path : List (SkolemFS sig)), path ∈ PreGroundTerm.function_paths_list ts -> ∀f, f ∈ path -> f ∈ FiniteTree.innerLabelsList ts := by
-      intro path path_mem f f_mem
-      cases ts with
-      | nil =>
-        unfold function_paths_list at path_mem
-        simp at path_mem
-      | cons hd tl =>
-        unfold function_paths_list at path_mem
-        rw [List.mem_append] at path_mem
-        unfold FiniteTree.innerLabelsList
-        rw [List.mem_append]
-        cases path_mem with
-        | inl path_mem =>
-          apply Or.inl
-          exact function_path_elements_are_inner_labels hd path path_mem f f_mem
-        | inr path_mem =>
-          apply Or.inr
-          exact function_path_elements_are_inner_labels_list tl path path_mem f f_mem
-
-  end
-
-  mutual
-
-    theorem PreGroundTerm.function_path_of_depth_exists (t : FiniteTree (SkolemFS sig) sig.C) : ∃ (path : List (SkolemFS sig)), path ∈ PreGroundTerm.function_paths t ∧ path.length = t.depth - 1 := by
-      cases t with
-      | leaf c => exists []; simp [FiniteTree.depth, function_paths]
-      | inner f ts =>
-        cases ts with
-        | nil =>
-          exists [f]
-          constructor
-          . unfold function_paths
-            simp
-          . unfold FiniteTree.depth
-            unfold FiniteTree.depthList
-            simp
-        | cons hd tl =>
-          rcases PreGroundTerm.function_path_of_depth_exists_list (FiniteTreeList.cons hd tl) (by simp) with ⟨path, mem, len⟩
-          exists (f :: path)
-          constructor
-          . unfold function_paths
-            rw [List.mem_map]
-            exists path
-          . unfold List.length
-            unfold FiniteTree.depth
-            rw [len]
-            rw [Nat.sub_one_add_one]
-            . rw [Nat.add_comm]
-              simp
-            . unfold FiniteTree.depthList
-              intro contra
-              have : hd.depth = 0 ∧ FiniteTree.depthList tl = 0 := by omega
-              have contra := this.left
-              unfold FiniteTree.depth at contra
-              cases hd <;> simp at contra
-
-    theorem PreGroundTerm.function_path_of_depth_exists_list (ts : FiniteTreeList (SkolemFS sig) sig.C) : ts ≠ FiniteTreeList.nil -> ∃ (path : List (SkolemFS sig)), path ∈ PreGroundTerm.function_paths_list ts ∧ path.length = (FiniteTree.depthList ts) - 1 := by
-      intro neq
-      cases ts with
-      | nil => simp at neq
-      | cons hd tl =>
-        cases tl with
-        | nil =>
-          have := function_path_of_depth_exists hd
-          rcases this with ⟨path, mem, len⟩
-          exists path
-          constructor
-          . unfold function_paths_list
-            rw [List.mem_append]
-            apply Or.inl
-            exact mem
-          . unfold FiniteTree.depthList
-            unfold FiniteTree.depthList
-            rw [Nat.max_eq_left]
-            . exact len
-            . unfold FiniteTree.depth
-              cases hd <;> simp
-        | cons mid tl =>
-          cases Decidable.em (hd.depth ≤ FiniteTree.depthList (FiniteTreeList.cons mid tl)) with
-          | inl depth_le =>
-            have := PreGroundTerm.function_path_of_depth_exists_list (FiniteTreeList.cons mid tl) (by simp)
-            rcases this with ⟨path, mem, len⟩
-            exists path
-            constructor
-            . unfold function_paths_list
-              rw [List.mem_append]
-              apply Or.inr
-              exact mem
-            . unfold FiniteTree.depthList
-              rw [Nat.max_eq_right]
-              . exact len
-              . exact depth_le
-          | inr depth_le =>
-            have := function_path_of_depth_exists hd
-            rcases this with ⟨path, mem, len⟩
-            exists path
-            constructor
-            . unfold function_paths_list
-              rw [List.mem_append]
-              apply Or.inl
-              exact mem
-            . unfold FiniteTree.depthList
-              rw [Nat.max_eq_left]
-              . exact len
-              . apply Nat.le_of_lt
-                simp at depth_le
-                exact depth_le
-
-  end
-
-  mutual
-
-    def PreGroundTerm.contains_func (func : SkolemFS sig) : FiniteTree (SkolemFS sig) sig.C -> Bool
-    | .leaf _ => false
-    | .inner func' ts => func == func' || PreGroundTerm.contains_func_list func ts
-
-    def PreGroundTerm.contains_func_list (func : SkolemFS sig) : FiniteTreeList (SkolemFS sig) sig.C -> Bool
-    | .nil => false
-    | .cons hd tl => contains_func func hd || contains_func_list func tl
-
-  end
-
-  mutual
-
-    theorem PreGroundTerm.function_path_elements_are_in_contains_func (t : FiniteTree (SkolemFS sig) sig.C) : ∀ (path : List (SkolemFS sig)), path ∈ PreGroundTerm.function_paths t -> ∀f, f ∈ path -> PreGroundTerm.contains_func f t := by
-      intro path path_mem f f_mem
-      cases t with
-      | leaf c =>
-        simp only [function_paths, List.mem_singleton] at path_mem
-        rw [path_mem] at f_mem
-        simp at f_mem
-      | inner func ts =>
-        unfold contains_func
-        rw [Bool.or_eq_true]
-        unfold function_paths at path_mem
-        cases ts with
-        | nil =>
-          rw [List.mem_singleton] at path_mem
-          rw [path_mem] at f_mem
-          rw [List.mem_singleton] at f_mem
-          apply Or.inl
-          rw [f_mem]
-          simp
-        | cons hd tl =>
-          rw [List.mem_map] at path_mem
-          rcases path_mem with ⟨path', mem, eq⟩
-          rw [← eq] at f_mem
-          rw [List.mem_cons] at f_mem
-          cases f_mem with
-          | inl f_mem => apply Or.inl; rw [f_mem]; simp
-          | inr f_mem =>
-            apply Or.inr
-            exact PreGroundTerm.function_path_elements_are_in_contains_func_list (FiniteTreeList.cons hd tl) path' mem f f_mem
-
-    theorem PreGroundTerm.function_path_elements_are_in_contains_func_list (ts : FiniteTreeList (SkolemFS sig) sig.C) : ∀ (path : List (SkolemFS sig)), path ∈ PreGroundTerm.function_paths_list ts -> ∀f, f ∈ path -> PreGroundTerm.contains_func_list f ts := by
-      intro path path_mem f f_mem
-      cases ts with
-      | nil =>
-        unfold function_paths_list at path_mem
-        simp at path_mem
-      | cons hd tl =>
-        unfold contains_func_list
-        rw [Bool.or_eq_true]
-        unfold function_paths_list at path_mem
-        rw [List.mem_append] at path_mem
-        cases path_mem with
-        | inl path_mem => apply Or.inl; exact function_path_elements_are_in_contains_func hd path path_mem f f_mem
-        | inr path_mem => apply Or.inr; exact function_path_elements_are_in_contains_func_list tl path path_mem f f_mem
-
-  end
-
-  mutual
-
-    def PreGroundTerm.cyclic : FiniteTree (SkolemFS sig) sig.C -> Bool
-    | .leaf _ => false
-    | .inner func ts => (contains_func_list func ts) || PreGroundTerm.cyclic_list ts
-
-    def PreGroundTerm.cyclic_list : FiniteTreeList (SkolemFS sig) sig.C -> Bool
-    | .nil => false
-    | .cons hd tl => PreGroundTerm.cyclic hd || PreGroundTerm.cyclic_list tl
-
-  end
-
-  mutual
-
-    theorem PreGroundTerm.cyclic_of_path_with_dup (t : FiniteTree (SkolemFS sig) sig.C) (path : List (SkolemFS sig)) (path_mem : path ∈ PreGroundTerm.function_paths t) (dup : ¬ path.Nodup) : PreGroundTerm.cyclic t := by
-      cases t with
-      | leaf c =>
-        unfold PreGroundTerm.function_paths at path_mem
-        rw [List.mem_singleton] at path_mem
-        rw [path_mem] at dup
-        simp at dup
-      | inner f ts =>
-        unfold PreGroundTerm.function_paths at path_mem
-        cases ts with
-        | nil =>
-          rw [List.mem_singleton] at path_mem
-          rw [path_mem] at dup
-          simp at dup
-        | cons hd tl =>
-          rw [List.mem_map] at path_mem
-          rcases path_mem with ⟨path', mem, eq⟩
-          unfold PreGroundTerm.cyclic
-          rw [Bool.or_eq_true]
-          cases Decidable.em (f ∈ path') with
-          | inl f_mem =>
-            apply Or.inl
-            exact PreGroundTerm.function_path_elements_are_in_contains_func_list (FiniteTreeList.cons hd tl) path' mem f f_mem
-          | inr f_mem =>
-            apply Or.inr
-            rw [← eq] at dup
-            rw [List.nodup_cons] at dup
-            simp only [not_and] at dup
-            apply PreGroundTerm.cyclic_of_path_with_dup_list (FiniteTreeList.cons hd tl) path' mem
-            apply dup
-            apply f_mem
-
-    theorem PreGroundTerm.cyclic_of_path_with_dup_list (ts : FiniteTreeList (SkolemFS sig) sig.C) (path : List (SkolemFS sig)) (path_mem : path ∈ PreGroundTerm.function_paths_list ts) (dup : ¬ path.Nodup) : PreGroundTerm.cyclic_list ts := by
-      unfold cyclic_list
-      cases ts with
-      | nil =>
-        unfold PreGroundTerm.function_paths_list at path_mem
-        simp at path_mem
-      | cons hd tl =>
-        unfold PreGroundTerm.function_paths_list at path_mem
-        rw [List.mem_append] at path_mem
-        rw [Bool.or_eq_true]
-        cases path_mem with
-        | inl path_mem =>
-          apply Or.inl
-          exact cyclic_of_path_with_dup hd path path_mem dup
-        | inr path_mem =>
-          apply Or.inr
-          exact cyclic_of_path_with_dup_list tl path path_mem dup
-
-  end
-
-  variable [DecidableEq sig.C]
-
-  theorem PreGroundTerm.cyclic_of_depth_too_big (t : PreGroundTerm sig) (funcs : List (SkolemFS sig)) (nodup : funcs.Nodup) (funcs_in_t_from_funcs : ∀ func, func ∈ t.innerLabels -> func ∈ funcs) : funcs.length + 2 ≤ t.depth -> PreGroundTerm.cyclic t := by
-    intro le_depth
-    have := PreGroundTerm.function_path_of_depth_exists t
-    rcases this with ⟨path, path_mem, path_len⟩
-
-    have path_length_gt : funcs.length < path.length := by
-      rw [path_len]
-      apply Nat.lt_of_succ_le
-      apply Nat.le_of_succ_le_succ
-      rw [Nat.succ_eq_add_one]
-      rw [Nat.succ_eq_add_one]
-      rw [Nat.sub_one_add_one]
-      . exact le_depth
-      . unfold FiniteTree.depth
-        cases t <;> simp
-
-    have dup_in_path : ¬ path.Nodup := by
-      apply List.contains_dup_of_exceeding_nodup_list_with_same_elements funcs path nodup path_length_gt
-      intro f f_mem
-      apply funcs_in_t_from_funcs
-      exact PreGroundTerm.function_path_elements_are_inner_labels t path path_mem f f_mem
-
-    exact PreGroundTerm.cyclic_of_path_with_dup t path path_mem dup_in_path
-
-end FunctionPathsAndCyclicity
+end PreGroundTerm
 
 abbrev GroundTerm (sig : Signature) [DecidableEq sig.C] [DecidableEq sig.V] := { t : PreGroundTerm sig // PreGroundTerm.arity_ok t }
 
 inductive SkolemTerm (sig : Signature) [DecidableEq sig.C] [DecidableEq sig.V] where
-  | var (v : sig.V) : SkolemTerm sig
-  | const (c : sig.C) : SkolemTerm sig
-  | func (fs : SkolemFS sig) (frontier : List sig.V) (arity_ok : frontier.length = fs.arity) : SkolemTerm sig
-  deriving DecidableEq
+| var (v : sig.V) : SkolemTerm sig
+| const (c : sig.C) : SkolemTerm sig
+| func (fs : SkolemFS sig) (frontier : List sig.V) (arity_ok : frontier.length = fs.arity) : SkolemTerm sig
+deriving DecidableEq
 
 inductive VarOrConst (sig : Signature) [DecidableEq sig.C] [DecidableEq sig.V] where
-  | var (v : sig.V) : VarOrConst sig
-  | const (c : sig.C) : VarOrConst sig
-  deriving DecidableEq
+| var (v : sig.V) : VarOrConst sig
+| const (c : sig.C) : VarOrConst sig
+deriving DecidableEq
 
 variable {sig : Signature} [DecidableEq sig.C] [DecidableEq sig.V]
 
-def GroundTerm.const (c : sig.C) : GroundTerm sig := ⟨FiniteTree.leaf c, by simp [PreGroundTerm.arity_ok]⟩
-def GroundTerm.func (func : SkolemFS sig) (ts : List (GroundTerm sig)) (arity_ok : ts.length = func.arity) : GroundTerm sig := ⟨FiniteTree.inner func (FiniteTreeList.fromList ts.unattach), by
-  unfold PreGroundTerm.arity_ok
-  rw [Bool.and_eq_true, beq_iff_eq]
-  rw [FiniteTreeList.fromListToListIsId]
-  constructor
-  . rw [List.length_unattach]; exact arity_ok
-  . rw [← PreGroundTerm.arity_ok_list_iff_arity_ok_each_mem]
+namespace GroundTerm
+
+  def const (c : sig.C) : GroundTerm sig := ⟨FiniteTree.leaf c, by simp [PreGroundTerm.arity_ok]⟩
+  def func (func : SkolemFS sig) (ts : List (GroundTerm sig)) (arity_ok : ts.length = func.arity) : GroundTerm sig := ⟨FiniteTree.inner func (FiniteTreeList.fromList ts.unattach), by
+    unfold PreGroundTerm.arity_ok
+    rw [Bool.and_eq_true, beq_iff_eq]
     rw [FiniteTreeList.fromListToListIsId]
-    intro t t_mem
-    unfold List.unattach at t_mem
-    rw [List.mem_map] at t_mem
-    rcases t_mem with ⟨t, t_mem, t_eq⟩
-    rw [← t_eq]
-    exact t.property
-⟩
+    constructor
+    . rw [List.length_unattach]; exact arity_ok
+    . rw [← PreGroundTerm.arity_ok_list_iff_arity_ok_each_mem]
+      rw [FiniteTreeList.fromListToListIsId]
+      intro t t_mem
+      unfold List.unattach at t_mem
+      rw [List.mem_map] at t_mem
+      rcases t_mem with ⟨t, t_mem, t_eq⟩
+      rw [← t_eq]
+      exact t.property
+  ⟩
 
--- TODO: we are barely using cases and rec for GroundTerm; use it more or remove it if it turns out to not be useful
-@[elab_as_elim, cases_eliminator]
-def GroundTerm.cases
-    {motive : GroundTerm sig -> Sort u}
-    (t : GroundTerm sig)
-    (const : (c : sig.C) -> (eq : t = GroundTerm.const c) -> motive (GroundTerm.const c))
-    (func : (func : SkolemFS sig) -> (ts : List (GroundTerm sig)) -> (arity_ok : ts.length = func.arity) -> (eq : t = GroundTerm.func func ts arity_ok) -> motive (GroundTerm.func func ts arity_ok)) :
-    motive t :=
-  match eq : t.val with
-  | .leaf c =>
-    have eq : t = GroundTerm.const c := Subtype.eq eq
-    eq ▸ const c eq
-  | .inner f ts => by
-    let ts : List (GroundTerm sig) := ts.toList.attach.map (fun ⟨t', mem⟩ => ⟨t', by
-      have prop := t.property
-      unfold PreGroundTerm.arity_ok at prop
-      simp only [eq, Bool.and_eq_true, beq_iff_eq] at prop
-      have prop := prop.right
-      rw [← PreGroundTerm.arity_ok_list_iff_arity_ok_each_mem] at prop
-      apply prop
-      exact mem
-    ⟩)
-    have arity_ok : ts.length = f.arity := by
-      have prop := t.property
-      unfold PreGroundTerm.arity_ok at prop
-      simp only [eq, Bool.and_eq_true, beq_iff_eq] at prop
-      unfold ts
-      rw [List.length_map, List.length_attach]
-      exact prop.left
-    have eq : t = GroundTerm.func f ts arity_ok := by
-      apply Subtype.eq
-      unfold GroundTerm.func
-      simp [eq, ts]
-      unfold List.unattach
-      rw [List.map_map, List.map_attach]
-      simp [FiniteTreeList.toListFromListIsId]
-    exact eq ▸ (func f ts arity_ok eq)
+  -- TODO: we are barely using cases and rec for GroundTerm; use it more or remove it if it turns out to not be useful
+  @[elab_as_elim, cases_eliminator]
+  def cases
+      {motive : GroundTerm sig -> Sort u}
+      (t : GroundTerm sig)
+      (const : (c : sig.C) -> motive (GroundTerm.const c))
+      (func : (func : SkolemFS sig) -> (ts : List (GroundTerm sig)) -> (arity_ok : ts.length = func.arity) -> motive (GroundTerm.func func ts arity_ok)) :
+      motive t :=
+    match eq : t.val with
+    | .leaf c =>
+      have eq : t = GroundTerm.const c := Subtype.eq eq
+      eq ▸ const c
+    | .inner f ts => by
+      let ts : List (GroundTerm sig) := ts.toList.attach.map (fun ⟨t', mem⟩ => ⟨t', by
+        have prop := t.property
+        unfold PreGroundTerm.arity_ok at prop
+        simp only [eq, Bool.and_eq_true, beq_iff_eq] at prop
+        have prop := prop.right
+        rw [← PreGroundTerm.arity_ok_list_iff_arity_ok_each_mem] at prop
+        apply prop
+        exact mem
+      ⟩)
+      have arity_ok : ts.length = f.arity := by
+        have prop := t.property
+        unfold PreGroundTerm.arity_ok at prop
+        simp only [eq, Bool.and_eq_true, beq_iff_eq] at prop
+        unfold ts
+        rw [List.length_map, List.length_attach]
+        exact prop.left
+      have eq : t = GroundTerm.func f ts arity_ok := by
+        apply Subtype.eq
+        unfold GroundTerm.func
+        simp [eq, ts]
+        unfold List.unattach
+        rw [List.map_map, List.map_attach]
+        simp [FiniteTreeList.toListFromListIsId]
+      exact eq ▸ (func f ts arity_ok)
 
-@[elab_as_elim, induction_eliminator]
-def GroundTerm.rec
-    {motive : GroundTerm sig -> Sort u}
-    (const : (c : sig.C) -> motive (GroundTerm.const c))
-    (func : (func : SkolemFS sig) -> (ts : List (GroundTerm sig)) -> (arity_ok : ts.length = func.arity) -> (∀ t, t ∈ ts -> motive t) -> motive (GroundTerm.func func ts arity_ok))
-    (t : GroundTerm sig) :
-    motive t :=
-  match eq_val : t.val with
-  | .leaf c =>
-    have eq : t = GroundTerm.const c := Subtype.eq eq_val
-    eq ▸ const c
-  | .inner f ts => by
-    let ts : List (GroundTerm sig) := ts.toList.attach.map (fun ⟨t', mem⟩ => ⟨t', by
-      have prop := t.property
-      unfold PreGroundTerm.arity_ok at prop
-      simp only [eq_val, Bool.and_eq_true, beq_iff_eq] at prop
-      have prop := prop.right
-      rw [← PreGroundTerm.arity_ok_list_iff_arity_ok_each_mem] at prop
-      apply prop
-      exact mem
-    ⟩)
-    have arity_ok : ts.length = f.arity := by
-      have prop := t.property
-      unfold PreGroundTerm.arity_ok at prop
-      simp only [eq_val, Bool.and_eq_true, beq_iff_eq] at prop
-      unfold ts
-      rw [List.length_map, List.length_attach]
-      exact prop.left
-    have eq : t = GroundTerm.func f ts arity_ok := by
-      apply Subtype.eq
-      unfold GroundTerm.func
-      simp [eq_val, ts]
-      unfold List.unattach
-      rw [List.map_map, List.map_attach]
-      simp [FiniteTreeList.toListFromListIsId]
-    exact eq ▸ (func f ts arity_ok (by
-      intro t' mem
-      have : t'.val.depth < t.val.depth := by
-        conv => right; unfold FiniteTree.depth
-        simp only [eq_val]
-        rw [Nat.add_comm]
-        apply Nat.lt_add_one_of_le
-        apply FiniteTree.depth_le_depthList_of_mem
-        unfold ts at mem
-        rw [List.mem_map] at mem
-        rcases mem with ⟨s, s_mem, t_eq⟩
-        simp at t_eq
-        rw [← t_eq]
-        unfold List.attach at s_mem
-        unfold List.attachWith at s_mem
-        rw [List.mem_pmap] at s_mem
-        rcases s_mem with ⟨_, s_mem, s_eq⟩
-        rw [← s_eq]
-        exact s_mem
-      apply GroundTerm.rec const func
-    ))
-termination_by t.val.depth
+  @[elab_as_elim, induction_eliminator]
+  def rec
+      {motive : GroundTerm sig -> Sort u}
+      (const : (c : sig.C) -> motive (GroundTerm.const c))
+      (func : (func : SkolemFS sig) -> (ts : List (GroundTerm sig)) -> (arity_ok : ts.length = func.arity) -> (∀ t, t ∈ ts -> motive t) -> motive (GroundTerm.func func ts arity_ok))
+      (t : GroundTerm sig) :
+      motive t :=
+    match eq_val : t.val with
+    | .leaf c =>
+      have eq : t = GroundTerm.const c := Subtype.eq eq_val
+      eq ▸ const c
+    | .inner f ts => by
+      let ts : List (GroundTerm sig) := ts.toList.attach.map (fun ⟨t', mem⟩ => ⟨t', by
+        have prop := t.property
+        unfold PreGroundTerm.arity_ok at prop
+        simp only [eq_val, Bool.and_eq_true, beq_iff_eq] at prop
+        have prop := prop.right
+        rw [← PreGroundTerm.arity_ok_list_iff_arity_ok_each_mem] at prop
+        apply prop
+        exact mem
+      ⟩)
+      have arity_ok : ts.length = f.arity := by
+        have prop := t.property
+        unfold PreGroundTerm.arity_ok at prop
+        simp only [eq_val, Bool.and_eq_true, beq_iff_eq] at prop
+        unfold ts
+        rw [List.length_map, List.length_attach]
+        exact prop.left
+      have eq : t = GroundTerm.func f ts arity_ok := by
+        apply Subtype.eq
+        unfold GroundTerm.func
+        simp [eq_val, ts]
+        unfold List.unattach
+        rw [List.map_map, List.map_attach]
+        simp [FiniteTreeList.toListFromListIsId]
+      exact eq ▸ (func f ts arity_ok (by
+        intro t' mem
+        have : t'.val.depth < t.val.depth := by
+          conv => right; unfold FiniteTree.depth
+          simp only [eq_val]
+          rw [Nat.add_comm]
+          apply Nat.lt_add_one_of_le
+          apply FiniteTree.depth_le_depthList_of_mem
+          unfold ts at mem
+          rw [List.mem_map] at mem
+          rcases mem with ⟨s, s_mem, t_eq⟩
+          simp at t_eq
+          rw [← t_eq]
+          unfold List.attach at s_mem
+          unfold List.attachWith at s_mem
+          rw [List.mem_pmap] at s_mem
+          rcases s_mem with ⟨_, s_mem, s_eq⟩
+          rw [← s_eq]
+          exact s_mem
+        apply GroundTerm.rec const func
+      ))
+  termination_by t.val.depth
 
-def GroundTerm.toConst (t : GroundTerm sig) (isConst : ∃ c, t = GroundTerm.const c) : sig.C :=
-  match eq : t.val with
-  | .leaf c => c
-  | .inner _ _ => by
-    apply False.elim
-    rcases isConst with ⟨c, isConst⟩
-    rw [isConst] at eq
-    simp [GroundTerm.const] at eq
+  def toConst (t : GroundTerm sig) (isConst : ∃ c, t = GroundTerm.const c) : sig.C :=
+    match eq : t.val with
+    | .leaf c => c
+    | .inner _ _ => by
+      apply False.elim
+      rcases isConst with ⟨c, isConst⟩
+      rw [isConst] at eq
+      simp [GroundTerm.const] at eq
 
-def SkolemTerm.variables : SkolemTerm sig -> List sig.V
+  def depth (t : GroundTerm sig) : Nat := t.val.depth
+  def constants (t : GroundTerm sig) : (List sig.C) := t.val.leaves
+  def functions (t : GroundTerm sig) : (List (SkolemFS sig)) := t.val.innerLabels
+
+  theorem depth_const (c : sig.C) : (GroundTerm.const c).depth = 1 := by
+    simp [GroundTerm.const, depth, FiniteTree.depth]
+
+  theorem depth_func (f : SkolemFS sig) (ts : List (GroundTerm sig)) (arity_ok : ts.length = f.arity) :
+      (GroundTerm.func f ts arity_ok).depth = 1 + (((ts.map (GroundTerm.depth)).max?).getD 1) := by
+    simp only [GroundTerm.func, depth, FiniteTree.depth]
+
+    have : ∀ (ts : List (GroundTerm sig)), (FiniteTree.depthList (FiniteTreeList.fromList ts.unattach)) = (((ts.map (GroundTerm.depth)).max?).getD 1) := by
+      intro ts
+      induction ts with
+      | nil => simp [FiniteTreeList.fromList, FiniteTree.depthList]
+      | cons hd tl ih =>
+        rw [List.map_cons, List.max?_cons, List.unattach_cons]
+        unfold FiniteTree.depthList
+        unfold FiniteTreeList.fromList
+        simp only [Option.getD_some]
+        cases eq : (tl.map depth).max? with
+        | some m => simp only [Option.elim]; rw [ih, eq, Option.getD_some]; rfl
+        | none =>
+          simp only [Option.elim]
+          rw [List.max?_eq_none_iff, List.map_eq_nil_iff] at eq
+          rw [eq]
+          simp only [FiniteTreeList.fromList, FiniteTree.depthList, List.unattach_nil]
+          rw [Nat.max_eq_left]
+          . rfl
+          . unfold FiniteTree.depth; cases hd.val <;> simp
+
+    rw [this]
+
+  theorem constants_const (c : sig.C) : (GroundTerm.const c).constants = [c] := by
+    simp [GroundTerm.const, constants, FiniteTree.leaves]
+
+  theorem constants_func (f : SkolemFS sig) (ts : List (GroundTerm sig)) (arity_ok : ts.length = f.arity) :
+      (GroundTerm.func f ts arity_ok).constants = ts.flatMap GroundTerm.constants := by
+    simp only [GroundTerm.func, constants, FiniteTree.leaves]
+
+    have : ∀ (ts : List (GroundTerm sig)), (FiniteTree.leavesList (FiniteTreeList.fromList ts.unattach)) = (ts.flatMap GroundTerm.constants) := by
+      intro ts
+      induction ts with
+      | nil => simp [FiniteTreeList.fromList, FiniteTree.leavesList]
+      | cons hd tl ih =>
+        rw [List.flatMap_cons, List.unattach_cons]
+        unfold FiniteTree.leavesList
+        unfold FiniteTreeList.fromList
+        simp only
+        rw [ih]
+        rfl
+
+    rw [this]
+
+  theorem functions_const (c : sig.C) : (GroundTerm.const c).functions = [] := by
+    simp [GroundTerm.const, functions, FiniteTree.innerLabels]
+
+  theorem functions_func (f : SkolemFS sig) (ts : List (GroundTerm sig)) (arity_ok : ts.length = f.arity) :
+      (GroundTerm.func f ts arity_ok).functions = f :: (ts.flatMap GroundTerm.functions) := by
+    simp only [GroundTerm.func, functions, FiniteTree.innerLabels]
+
+    have : ∀ (ts : List (GroundTerm sig)), (FiniteTree.innerLabelsList (FiniteTreeList.fromList ts.unattach)) = (ts.flatMap GroundTerm.functions) := by
+      intro ts
+      induction ts with
+      | nil => simp [FiniteTreeList.fromList, FiniteTree.innerLabelsList]
+      | cons hd tl ih =>
+        rw [List.flatMap_cons, List.unattach_cons]
+        unfold FiniteTree.innerLabelsList
+        unfold FiniteTreeList.fromList
+        simp only
+        rw [ih]
+        rfl
+
+    rw [this]
+
+end GroundTerm
+
+namespace SkolemTerm
+
+  def variables : SkolemTerm sig -> List sig.V
   | .var v => List.cons v List.nil
   | .const _ => List.nil
   | .func _ vs _ => vs
+
+end SkolemTerm
 
 namespace VarOrConst
 
@@ -600,375 +370,4 @@ namespace VarOrConst
       | const _ => simp [skolemize]
 
 end VarOrConst
-
-
-section ListsOfTerms
-
-  variable {sig : Signature} [DecidableEq sig.C] [DecidableEq sig.V]
-
-  def all_term_lists_of_length (candidate_terms : List (GroundTerm sig)) : Nat -> List (List (GroundTerm sig))
-  | .zero => [[]]
-  | .succ n =>
-    let prev_terms := all_term_lists_of_length candidate_terms n
-    candidate_terms.flatMap (fun t =>
-      prev_terms.map (fun ts =>
-        t :: ts
-      )
-    )
-
-  theorem mem_all_term_lists_of_length (candidate_terms : List (GroundTerm sig)) (length : Nat) : ∀ ts, ts ∈ (all_term_lists_of_length candidate_terms length) ↔ (ts.length = length ∧ (∀ t, t ∈ ts -> t ∈ candidate_terms)) := by
-    induction length with
-    | zero => intro ts; unfold all_term_lists_of_length; simp; intro eq t _ mem; rw [eq] at mem; simp at mem
-    | succ length ih =>
-      intro ts
-      unfold all_term_lists_of_length
-      simp only [List.mem_flatMap, List.mem_map]
-
-      constructor
-      . intro h
-        rcases h with ⟨t, t_mem, prev, prev_mem, ts_eq⟩
-        rw [← ts_eq]
-        specialize ih prev
-        have ih := ih.mp prev_mem
-        constructor
-        . rw [List.length_cons, ih.left]
-        . intro t' t'_mem
-          rw [List.mem_cons] at t'_mem
-          cases t'_mem with
-          | inl t'_mem => rw [t'_mem]; apply t_mem
-          | inr t'_mem => apply ih.right; exact t'_mem
-      . intro h
-        cases ts with
-        | nil => simp at h
-        | cons hd tl =>
-          exists hd
-          constructor
-          . apply h.right
-            simp
-          . exists tl
-            constructor
-            . rw [ih]
-              constructor
-              . have l := h.left
-                rw [List.length_cons, Nat.add_right_cancel_iff] at l
-                exact l
-              . intro t t_mem
-                apply h.right
-                simp [t_mem]
-            . rfl
-
-  def all_terms_limited_by_depth (constants : List sig.C) (funcs : List (SkolemFS sig)) : Nat -> List (GroundTerm sig)
-  | 0 => []
-  | 1 => constants.map GroundTerm.const
-  | .succ (.succ depth) =>
-    let prev := all_terms_limited_by_depth constants funcs (.succ depth)
-    funcs.flatMap (fun func =>
-      (all_term_lists_of_length prev func.arity).attach.map (fun ⟨ts, mem⟩ =>
-        ⟨
-          FiniteTree.inner func (FiniteTreeList.fromList ts.unattach),
-          by
-            unfold PreGroundTerm.arity_ok
-            simp
-            constructor
-            . rw [FiniteTreeList.fromListToListIsId]
-              rw [List.length_unattach]
-              rw [mem_all_term_lists_of_length] at mem
-              exact mem.left
-            . apply (PreGroundTerm.arity_ok_list_iff_arity_ok_each_mem _).mp
-              rw [FiniteTreeList.fromListToListIsId]
-              intro t t_mem
-              unfold List.unattach at t_mem
-              rw [List.mem_map] at t_mem
-              rcases t_mem with ⟨t, h⟩
-              rw [← h.right]
-              exact t.property
-        ⟩
-      )
-    ) ++ prev
-
-  theorem mem_all_terms_limited_by_depth (constants : List sig.C) (funcs : List (SkolemFS sig)) (depth : Nat) :
-      ∀ t, t ∈ (all_terms_limited_by_depth constants funcs depth) ↔ (t.val.depth ≤ depth ∧ (∀ c, c ∈ t.val.leaves -> c ∈ constants) ∧ (∀ func, func ∈ t.val.innerLabels -> func ∈ funcs)) := by
-    induction depth with
-    | zero =>
-      simp [all_terms_limited_by_depth]
-      intro t _ t_depth
-      cases t <;> simp [FiniteTree.depth] at t_depth
-    | succ depth ih =>
-      intro t
-      unfold all_terms_limited_by_depth
-
-      cases depth with
-      | zero =>
-        simp only [Nat.zero_add]
-        constructor
-        . intro h
-          rw [List.mem_map] at h
-          rcases h with ⟨c, c_mem, h⟩
-          rw [← h]
-          simp [GroundTerm.const, FiniteTree.depth, FiniteTree.leaves, FiniteTree.innerLabels]
-          exact c_mem
-        . intro h
-          cases eq : t with
-          | const c =>
-            rw [List.mem_map]
-            exists c
-            constructor
-            . apply h.right.left
-              simp [eq, GroundTerm.const, FiniteTree.leaves]
-            . rfl
-          | func _ ts _ =>
-            have contra := h.left
-            unfold FiniteTree.depth at contra
-            simp only [eq, GroundTerm.func] at contra
-            cases ts with
-            | nil => simp [FiniteTreeList.fromList, FiniteTree.depthList] at contra
-            | cons t _ =>
-              simp only [List.unattach, List.map_cons, FiniteTreeList.fromList, FiniteTree.depthList] at contra
-              rw [Nat.add_comm, Nat.succ_le_succ_iff, Nat.max_le] at contra
-              have contra := contra.left
-              unfold FiniteTree.depth at contra
-              cases eq : t.val <;> simp [eq] at contra
-      | succ depth =>
-        let rec aux : ∀ (ts : FiniteTreeList (SkolemFS sig) sig.C), (PreGroundTerm.arity_ok_list ts) -> ((∀ (t : GroundTerm sig), t.val ∈ ts.toList -> t ∈ (all_terms_limited_by_depth constants funcs depth.succ)) ↔
-            ((FiniteTree.depthList ts ≤ depth.succ) ∧ (∀ c, c ∈ FiniteTree.leavesList ts -> c ∈ constants) ∧ (∀ func, func ∈ FiniteTree.innerLabelsList ts -> func ∈ funcs))) := by
-          intro ts arities_ok
-          cases ts with
-          | nil =>
-            simp [FiniteTree.depthList, FiniteTree.leavesList, FiniteTree.innerLabelsList, FiniteTreeList.toList]
-          | cons hd tl =>
-            unfold PreGroundTerm.arity_ok_list at arities_ok
-            rw [Bool.and_eq_true] at arities_ok
-            unfold FiniteTree.depthList
-            unfold FiniteTree.leavesList
-            unfold FiniteTree.innerLabelsList
-
-            specialize ih ⟨hd, arities_ok.left⟩
-            have ih_inner := aux tl
-
-            constructor
-            . intro h
-
-              have ih := ih.mp (by
-                apply h
-                unfold FiniteTreeList.toList
-                simp
-              )
-              have ih_inner := (ih_inner arities_ok.right).mp (by
-                intro t t_mem
-                apply h
-                unfold FiniteTreeList.toList
-                simp [t_mem]
-              )
-
-              constructor
-              . rw [Nat.max_le]
-                constructor
-                . apply ih.left
-                . apply ih_inner.left
-              constructor
-              . intro c c_mem
-                rw [List.mem_append] at c_mem
-                cases c_mem with
-                | inl c_mem => apply ih.right.left; exact c_mem
-                | inr c_mem => apply ih_inner.right.left; exact c_mem
-              . intro func func_mem
-                rw [List.mem_append] at func_mem
-                cases func_mem with
-                | inl func_mem => apply ih.right.right; exact func_mem
-                | inr func_mem => apply ih_inner.right.right; exact func_mem
-            . intro h
-              rw [Nat.max_le] at h
-
-              have ih := ih.mpr (by
-                constructor
-                . exact h.left.left
-                constructor
-                . intro c c_mem
-                  apply h.right.left
-                  rw [List.mem_append]
-                  apply Or.inl
-                  exact c_mem
-                . intro func func_mem
-                  apply h.right.right
-                  rw [List.mem_append]
-                  apply Or.inl
-                  exact func_mem
-              )
-              have ih_inner := (ih_inner arities_ok.right).mpr (by
-                constructor
-                . exact h.left.right
-                constructor
-                . intro c c_mem
-                  apply h.right.left
-                  rw [List.mem_append]
-                  apply Or.inr
-                  exact c_mem
-                . intro func func_mem
-                  apply h.right.right
-                  rw [List.mem_append]
-                  apply Or.inr
-                  exact func_mem
-              )
-              intro t t_mem
-              unfold FiniteTreeList.toList at t_mem
-              rw [List.mem_cons] at t_mem
-              cases t_mem with
-              | inl t_mem =>
-                have : t = ⟨hd, arities_ok.left⟩ := by apply Subtype.eq; exact t_mem
-                rw [this]
-                apply ih
-              | inr t_mem => apply ih_inner; exact t_mem
-
-        constructor
-        . intro h
-          rw [List.mem_append] at h
-          cases h with
-          | inr h =>
-            rw [ih] at h
-            constructor
-            . apply Nat.le_succ_of_le
-              exact h.left
-            constructor
-            . exact h.right.left
-            . exact h.right.right
-          | inl h =>
-            simp only [List.mem_flatMap, List.mem_map] at h
-            rcases h with ⟨func, func_mem, ts, ts_mem, t_eq⟩
-            rw [← t_eq]
-            unfold List.attach at ts_mem
-            unfold List.attachWith at ts_mem
-            rw [List.mem_pmap] at ts_mem
-            rcases ts_mem with ⟨ts_val, ts_mem, ts_eq⟩
-            rw [mem_all_term_lists_of_length] at ts_mem
-
-            unfold FiniteTree.depth
-            unfold FiniteTree.leaves
-            unfold FiniteTree.innerLabels
-
-            have this := (aux (FiniteTreeList.fromList ts_val.unattach) (by
-              apply (PreGroundTerm.arity_ok_list_iff_arity_ok_each_mem _).mp
-              rw [FiniteTreeList.fromListToListIsId]
-              intro t t_mem
-              unfold List.unattach at t_mem
-              rw [List.mem_map] at t_mem
-              rcases t_mem with ⟨t, h⟩
-              rw [← h.right]
-              exact t.property
-            )).mp (by
-              intro t t_mem
-              rw [FiniteTreeList.fromListToListIsId] at t_mem
-              apply ts_mem.right
-              unfold List.unattach at t_mem
-              rw [List.mem_map] at t_mem
-              rcases t_mem with ⟨t', mem, eq⟩
-              have : t' = t := by apply Subtype.eq; exact eq
-              rw [← this]
-              exact mem
-            )
-
-            rw [← ts_eq]
-            constructor
-            . rw [Nat.add_comm]
-              apply Nat.succ_le_succ
-              exact this.left
-            constructor
-            . exact this.right.left
-            . intro func' func'_mem
-              rw [List.mem_cons] at func'_mem
-              cases func'_mem with
-              | inl func'_mem => rw [func'_mem]; exact func_mem
-              | inr func'_mem => apply this.right.right; exact func'_mem
-
-        . intro h
-          rw [List.mem_append]
-          simp only [List.mem_flatMap, List.mem_map]
-          rcases h with ⟨depth_le, consts_mem, funcs_mem⟩
-          rw [Nat.le_iff_lt_or_eq] at depth_le
-          cases depth_le with
-          | inl depth_le =>
-            apply Or.inr
-            rw [ih]
-            constructor
-            . apply Nat.le_of_lt_succ
-              exact depth_le
-            constructor
-            . exact consts_mem
-            . exact funcs_mem
-          | inr depth_le =>
-            cases eq : t.val with
-            | leaf _ => rw [eq] at depth_le; simp [FiniteTree.depth] at depth_le
-            | inner t_func ts =>
-              rw [eq] at depth_le
-              rw [eq] at consts_mem
-              rw [eq] at funcs_mem
-              unfold FiniteTree.depth at depth_le
-              unfold FiniteTree.leaves at consts_mem
-              unfold FiniteTree.innerLabels at funcs_mem
-
-              have this := (aux ts (by have prop := t.property; unfold PreGroundTerm.arity_ok at prop; simp only [eq, Bool.and_eq_true] at prop; exact prop.right)).mpr (by
-                constructor
-                . apply Nat.le_of_eq
-                  rw [Nat.add_comm] at depth_le
-                  injection depth_le with depth_le
-                constructor
-                . exact consts_mem
-                . intro func func_mem
-                  apply funcs_mem
-                  simp [func_mem]
-              )
-
-              apply Or.inl
-              exists t_func
-              constructor
-              . apply funcs_mem
-                simp
-              let ts_ground_terms : List (GroundTerm sig) := ts.toList.attach.map (fun ⟨t', mem⟩ =>
-                ⟨t', by
-                  have prop := t.property
-                  unfold PreGroundTerm.arity_ok at prop
-                  rw [eq] at prop
-                  simp only [Bool.and_eq_true] at prop
-                  apply (PreGroundTerm.arity_ok_list_iff_arity_ok_each_mem ts).mpr
-                  . exact prop.right
-                  . exact mem
-                ⟩
-              )
-              have : ts_ground_terms ∈ all_term_lists_of_length (all_terms_limited_by_depth constants funcs depth.succ) t_func.arity := by
-                rw [mem_all_term_lists_of_length]
-                constructor
-                . have prop := t.property
-                  unfold PreGroundTerm.arity_ok at prop
-                  rw [eq, Bool.and_eq_true, beq_iff_eq] at prop
-                  unfold ts_ground_terms
-                  rw [List.length_map, List.length_attach]
-                  exact prop.left
-                . intro t t_mem
-                  apply this
-                  unfold ts_ground_terms at t_mem
-                  rw [List.mem_map] at t_mem
-                  rcases t_mem with ⟨val, val_mem, t_eq⟩
-                  unfold List.attach at val_mem
-                  unfold List.attachWith at val_mem
-                  rw [List.mem_pmap] at val_mem
-                  rcases val_mem with ⟨_, val_mem, eq⟩
-                  simp only at t_eq
-                  rw [← t_eq, ← eq]
-                  exact val_mem
-
-              exists ⟨ts_ground_terms, this⟩
-
-              constructor
-              . apply List.mem_attach
-              . have : ts_ground_terms.unattach = ts.toList := by
-                  unfold List.unattach
-                  unfold ts_ground_terms
-                  rw [List.map_map, List.map_attach]
-                  simp
-                apply Subtype.eq
-                simp only
-                rw [this]
-                rw [FiniteTreeList.toListFromListIsId]
-                rw [eq]
-
-end ListsOfTerms
 
