ExistentialRules/Terms/ListsOfTerms.lean
@@ -1,0 +1,309 @@
+import ExistentialRules.Terms.Basic
+
+variable {sig : Signature} [DecidableEq sig.C] [DecidableEq sig.V]
+
+def all_term_lists_of_length (candidate_terms : List (GroundTerm sig)) : Nat -> List (List (GroundTerm sig))
+| .zero => [[]]
+| .succ n =>
+  let prev_terms := all_term_lists_of_length candidate_terms n
+  candidate_terms.flatMap (fun t =>
+    prev_terms.map (fun ts =>
+      t :: ts
+    )
+  )
+
+theorem mem_all_term_lists_of_length (candidate_terms : List (GroundTerm sig)) (length : Nat) : ∀ ts, ts ∈ (all_term_lists_of_length candidate_terms length) ↔ (ts.length = length ∧ (∀ t, t ∈ ts -> t ∈ candidate_terms)) := by
+  induction length with
+  | zero => intro ts; unfold all_term_lists_of_length; simp; intro eq t _ mem; rw [eq] at mem; simp at mem
+  | succ length ih =>
+    intro ts
+    unfold all_term_lists_of_length
+    simp only [List.mem_flatMap, List.mem_map]
+
+    constructor
+    . intro h
+      rcases h with ⟨t, t_mem, prev, prev_mem, ts_eq⟩
+      rw [← ts_eq]
+      specialize ih prev
+      have ih := ih.mp prev_mem
+      constructor
+      . rw [List.length_cons, ih.left]
+      . intro t' t'_mem
+        rw [List.mem_cons] at t'_mem
+        cases t'_mem with
+        | inl t'_mem => rw [t'_mem]; apply t_mem
+        | inr t'_mem => apply ih.right; exact t'_mem
+    . intro h
+      cases ts with
+      | nil => simp at h
+      | cons hd tl =>
+        exists hd
+        constructor
+        . apply h.right
+          simp
+        . exists tl
+          constructor
+          . rw [ih]
+            constructor
+            . have l := h.left
+              rw [List.length_cons, Nat.add_right_cancel_iff] at l
+              exact l
+            . intro t t_mem
+              apply h.right
+              simp [t_mem]
+          . rfl
+
+def all_terms_limited_by_depth (constants : List sig.C) (funcs : List (SkolemFS sig)) : Nat -> List (GroundTerm sig)
+| 0 => []
+| 1 => constants.map GroundTerm.const
+| .succ (.succ depth) =>
+  let prev := all_terms_limited_by_depth constants funcs (.succ depth)
+  funcs.flatMap (fun func =>
+    (all_term_lists_of_length prev func.arity).attach.map (fun ⟨ts, mem⟩ =>
+      GroundTerm.func func ts (by
+        rw [mem_all_term_lists_of_length] at mem
+        exact mem.left
+      )
+    )
+  ) ++ prev
+
+theorem mem_all_terms_limited_by_depth (constants : List sig.C) (funcs : List (SkolemFS sig)) (depth : Nat) :
+    ∀ t, t ∈ (all_terms_limited_by_depth constants funcs depth) ↔ (t.depth ≤ depth ∧ (∀ c, c ∈ t.constants -> c ∈ constants) ∧ (∀ func, func ∈ t.functions -> func ∈ funcs)) := by
+  induction depth with
+  | zero =>
+    simp [all_terms_limited_by_depth]
+    intro t _ t_depth
+    cases t <;> simp [GroundTerm.depth, FiniteTree.depth] at t_depth
+  | succ depth ih =>
+    intro t
+    unfold all_terms_limited_by_depth
+
+    cases depth with
+    | zero =>
+      simp only [Nat.zero_add]
+      constructor
+      . intro h
+        rw [List.mem_map] at h
+        rcases h with ⟨c, c_mem, h⟩
+        rw [← h]
+        rw [GroundTerm.depth_const]
+        rw [GroundTerm.constants_const]
+        rw [GroundTerm.functions_const]
+        simp [c_mem]
+      . intro h
+        cases eq : t with
+        | const c =>
+          rw [List.mem_map]
+          exists c
+          constructor
+          . apply h.right.left
+            simp [eq, GroundTerm.constants_const]
+          . rfl
+        | func _ ts _ =>
+          have contra := h.left
+          rw [eq, GroundTerm.depth_func] at contra
+          cases eq : (ts.map GroundTerm.depth).max? with
+          | none => simp [eq] at contra
+          | some m =>
+            cases m with
+            | zero =>
+              rw [List.max?_eq_some_iff] at eq
+              . have contra := eq.left
+                rw [List.mem_map] at contra
+                rcases contra with ⟨t, t_mem, contra⟩
+                cases t <;> simp [GroundTerm.depth_const, GroundTerm.depth_func] at contra
+              . simp
+              . intro a b; cases Decidable.em (a ≤ b) with
+                | inl le => apply Or.inr; apply Nat.max_eq_right; exact le
+                | inr le => apply Or.inl; apply Nat.max_eq_left; apply Nat.le_of_not_le; exact le
+              . intros; apply Nat.max_le
+            | succ m =>
+              rw [eq, Nat.add_comm] at contra
+              simp at contra
+
+    | succ depth =>
+      have aux : ∀ (ts : List (GroundTerm sig)),
+          ((∀ (t : GroundTerm sig), t ∈ ts -> t ∈ (all_terms_limited_by_depth constants funcs depth.succ)) ↔
+          ((ts.all (fun t => t.depth ≤ depth.succ)) ∧ (∀ c, c ∈ (ts.flatMap GroundTerm.constants) -> c ∈ constants) ∧ (∀ func, func ∈ (ts.flatMap GroundTerm.functions) -> func ∈ funcs))) := by
+        intro ts
+        induction ts with
+        | nil => simp
+        | cons hd tl ih_inner =>
+          simp only [List.mem_cons, List.all_cons, Bool.and_eq_true, decide_eq_true_eq, List.flatMap_cons, List.mem_append]
+          constructor
+          . intro h
+            have ih := (ih hd).mp (by apply h; simp)
+            have ih_inner := ih_inner.mp (by intro _ t_mem; apply h; apply Or.inr; exact t_mem)
+            constructor
+            . constructor
+              . exact ih.left
+              . exact ih_inner.left
+            constructor
+            . intro c c_mem
+              cases c_mem with
+              | inl c_mem => apply ih.right.left; exact c_mem
+              | inr c_mem => apply ih_inner.right.left; exact c_mem
+            . intro f f_mem
+              cases f_mem with
+              | inl f_mem => apply ih.right.right; exact f_mem
+              | inr f_mem => apply ih_inner.right.right; exact f_mem
+          . intro h
+            intro t t_mem
+            cases t_mem with
+            | inl t_mem =>
+              rw [t_mem, ih]
+              constructor
+              . exact h.left.left
+              constructor
+              . intro c c_mem
+                apply h.right.left
+                apply Or.inl
+                exact c_mem
+              . intro f f_mem
+                apply h.right.right
+                apply Or.inl
+                exact f_mem
+            | inr t_mem =>
+              apply ih_inner.mpr
+              . constructor
+                . exact h.left.right
+                constructor
+                . intro c c_mem
+                  apply h.right.left
+                  apply Or.inr
+                  exact c_mem
+                . intro f f_mem
+                  apply h.right.right
+                  apply Or.inr
+                  exact f_mem
+              . exact t_mem
+
+      constructor
+      . intro h
+        rw [List.mem_append] at h
+        cases h with
+        | inr h =>
+          rw [ih] at h
+          constructor
+          . apply Nat.le_succ_of_le
+            exact h.left
+          constructor
+          . exact h.right.left
+          . exact h.right.right
+        | inl h =>
+          simp only [List.mem_flatMap, List.mem_map] at h
+          rcases h with ⟨func, func_mem, ts, ts_mem, t_eq⟩
+          rw [← t_eq]
+          unfold List.attach at ts_mem
+          unfold List.attachWith at ts_mem
+          rw [List.mem_pmap] at ts_mem
+          rcases ts_mem with ⟨ts_val, ts_mem, ts_eq⟩
+          rw [mem_all_term_lists_of_length] at ts_mem
+
+          rw [GroundTerm.depth_func]
+          rw [GroundTerm.constants_func]
+          rw [GroundTerm.functions_func]
+
+          have this := (aux ts_val).mp (by
+            intro t t_mem
+            apply ts_mem.right
+            exact t_mem
+          )
+
+          rw [← ts_eq]
+          constructor
+          . rw [Nat.add_comm]
+            apply Nat.succ_le_succ
+            cases eq : (ts_val.map GroundTerm.depth).max? with
+            | none => simp
+            | some m =>
+              rw [Option.getD_some, (ts_val.map GroundTerm.depth).max?_le_iff]
+              have depth_ts := List.all_eq_true.mp this.left
+              . simp only [decide_eq_true_iff] at depth_ts
+                intro d d_mem
+                rw [List.mem_map] at d_mem
+                rcases d_mem with ⟨t, t_mem, d_mem⟩
+                rw [← d_mem]
+                apply depth_ts
+                exact t_mem
+              . intros; apply Nat.max_le
+              . exact eq
+          constructor
+          . exact this.right.left
+          . intro func' func'_mem
+            rw [List.mem_cons] at func'_mem
+            cases func'_mem with
+            | inl func'_mem => rw [func'_mem]; exact func_mem
+            | inr func'_mem => apply this.right.right; exact func'_mem
+
+      . intro h
+        rw [List.mem_append]
+        simp only [List.mem_flatMap, List.mem_map]
+        rcases h with ⟨depth_le, consts_mem, funcs_mem⟩
+        rw [Nat.le_iff_lt_or_eq] at depth_le
+        cases depth_le with
+        | inl depth_le =>
+          apply Or.inr
+          rw [ih]
+          constructor
+          . apply Nat.le_of_lt_succ
+            exact depth_le
+          constructor
+          . exact consts_mem
+          . exact funcs_mem
+        | inr depth_le =>
+          cases eq : t with
+          | const _ => rw [eq] at depth_le; simp [GroundTerm.depth_const] at depth_le
+          | func t_func ts =>
+            rw [eq, GroundTerm.depth_func] at depth_le
+            rw [eq, GroundTerm.constants_func] at consts_mem
+            rw [eq, GroundTerm.functions_func] at funcs_mem
+            rw [Nat.add_comm, Nat.add_right_cancel_iff] at depth_le
+
+            have this := (aux ts).mpr (by
+              constructor
+              . rw [List.all_eq_true]
+                intro t t_mem
+                rw [decide_eq_true_iff]
+                cases eq : (ts.map GroundTerm.depth).max? with
+                | none => rw [List.max?_eq_none_iff, List.map_eq_nil_iff] at eq; rw [eq] at t_mem; simp at t_mem
+                | some m =>
+                  rw [eq, Option.getD_some, ← Nat.succ_eq_add_one] at depth_le
+                  rw [List.max?_eq_some_iff] at eq
+                  . rw [← depth_le]
+                    apply eq.right
+                    rw [List.mem_map]
+                    exists t
+                  . simp
+                  . intro a b; cases Decidable.em (a ≤ b) with
+                    | inl le => apply Or.inr; apply Nat.max_eq_right; exact le
+                    | inr le => apply Or.inl; apply Nat.max_eq_left; apply Nat.le_of_not_le; exact le
+                  . intros; apply Nat.max_le
+              constructor
+              . exact consts_mem
+              . intro func func_mem
+                apply funcs_mem
+                simp [func_mem]
+            )
+
+            apply Or.inl
+            exists t_func
+            constructor
+            . apply funcs_mem
+              simp
+
+            have ts_mem : ts ∈ all_term_lists_of_length (all_terms_limited_by_depth constants funcs depth.succ) t_func.arity := by
+              rw [mem_all_term_lists_of_length]
+              constructor
+              . have prop := t.property
+                unfold PreGroundTerm.arity_ok at prop
+                simp only [eq, GroundTerm.func, Bool.and_eq_true, beq_iff_eq] at prop
+                rw [FiniteTreeList.fromListToListIsId, List.length_unattach] at prop
+                exact prop.left
+              . intro t t_mem
+                apply this
+                exact t_mem
+
+            exists ⟨ts, ts_mem⟩
+            simp
+
